platform/cito/GoodOptimizer.v
@@ -1,5 +1,6 @@
 Require Import Syntax Semantics.
 Require Import CompileStatement.
+Require Import GeneralTactics.
 
 Set Implicit Arguments.
 
@@ -9,3 +10,25 @@ Definition is_good_optimizer optimizer :=
   (forall s, List.incl (SemanticsLemmas.footprint (optimizer s)) (SemanticsLemmas.footprint s)) /\
   (forall s, CompileStatement.depth (optimizer s) <= CompileStatement.depth s).
 
+Definition compose A B C (g : B -> C) (f : A -> B) x := g (f x).
+
+Lemma is_good_optimizer_trans : 
+  forall a b,
+    is_good_optimizer a ->
+    is_good_optimizer b ->
+    is_good_optimizer (compose a b).
+Proof.
+  unfold is_good_optimizer, compose; intros.
+
+  openhyp.
+  repeat split.
+  intros.
+  eapply H in H7; eauto; openhyp.
+  eapply H0 in H7; eauto; openhyp.
+
+  eauto.
+
+  eauto.
+
+  eauto using Le.le_trans.
+Qed.
